LocalLang/SemanticsExamples.lean
@@ -1,0 +1,89 @@
+import LocalLang.Semantics
+import LocalLang.SemanticsLemmas
+import LocalLang.Ctx
+import Mathlib.Data.List.Sigma
+import Std.Data.HashMap.Basic
+import Std.Data.HashMap.Lemmas
+
+instance : Add Expr where
+  add := .binOp .add
+
+instance : Coe String Expr where
+  coe := .var
+
+instance : OfNat Expr n where
+  ofNat := .const n
+
+abbrev f_body : Expr := (.funCall "g" [ "x" + 1 ]) + "x"
+abbrev f : Function := {
+  parameters := ["x"],
+  body := f_body
+}
+abbrev g : Function := {
+  parameters := ["x"],
+  body := "x"
+}
+
+abbrev defs := Std.HashMap.ofList [("f", f), ("g", g)]
+
+@[simp] lemma defs_f : defs["f"] = f := by
+  apply (Std.HashMap.getElem_ofList_of_mem (k := "f")) <;> simp
+@[simp] lemma defs_g : defs["g"] = g := by
+  apply (Std.HashMap.getElem_ofList_of_mem (k := "g")) <;> simp
+
+lemma f_steps
+  : SmallSteps defs (Std.HashMap.ofList [("x", 0)])
+      (Expr.funCall "g" ["x" + 1] + Expr.var "x") 1 := by
+  let locals := Std.HashMap.ofList [("x", 0)]
+  calc
+    SmallSteps defs locals _ (1 + "x") := by
+      apply (SmallSteps.with_ctx (.binOpLhs .hole .add "x") rfl rfl)
+      simp only [Ctx.updateEnv]
+      calc
+        SmallStep defs locals _ (.letIn "x" ("x" + 1) "x") := by
+          apply SmallStep.hole_step
+          apply (HeadSmallStep.fun_step ?_ rfl) <;> try rw [defs_g]
+          · simp
+          · rfl
+          · simp
+        SmallSteps defs locals _ (.letIn "x" 1 "x") := by
+          apply (SmallSteps.with_ctx (.letInExpr "x" .hole "x") rfl rfl)
+          calc
+            SmallStep defs locals _ ((0 : Expr) + 1) := by
+              apply (SmallStep.ctx_step (.binOpLhs .hole .add 1) rfl rfl)
+              constructor
+              simp [locals]
+            SmallStep defs locals _ _ := by
+              apply SmallStep.hole_step
+              constructor
+              rfl
+        SmallStep defs locals _ (.letIn "x" 1 1) := by
+          apply (SmallStep.ctx_step (.letInBody "x" 1 .hole) rfl rfl)
+          constructor
+          simp
+        SmallStep defs locals _ 1 := by
+          apply SmallStep.hole_step
+          constructor
+    SmallStep defs locals _ ((1 : Expr) + 0) := by
+      apply (SmallStep.ctx_step (.binOpRhs 1 .add .hole) rfl rfl)
+      constructor
+      simp [locals]
+    SmallStep defs locals _ _ := by
+      apply SmallStep.hole_step
+      constructor
+      rfl
+
+example : SmallSteps defs ∅ (.funCall "f" [0]) 1 := by
+  calc
+    SmallStep defs ∅ _ (.letIn "x" 0 f_body) := by
+      apply SmallStep.hole_step
+      apply (HeadSmallStep.fun_step ?_ rfl) <;> try rw [defs_f]
+      · simp
+      · rfl
+      · simp
+    SmallSteps defs ∅ _ (.letIn "x" 0 1) := by
+      apply (SmallSteps.with_ctx (.letInBody "x" 0 .hole) rfl rfl)
+      exact f_steps
+    SmallStep defs ∅ _ _ := by
+      apply SmallStep.hole_step
+      constructor
