LocalLang/SemanticsLemmas.lean
@@ -1,18 +1,21 @@
 import LocalLang.Semantics
 
-instance {defs : Definitions} :
+variable {defs : Definitions}
+
+instance :
   Trans (SmallStep defs V) (SmallStep defs V) (SmallSteps defs V) where
     trans st₁ st₂ := Relation.ReflTransGen.trans
       (Relation.ReflTransGen.single st₁) (Relation.ReflTransGen.single st₂)
 
-lemma head_step_implies_context_step {e₁ e₂ e₁' e₂' : Expr} {V V' : Env} {defs : Definitions}
-  (st : HeadSmallStep defs V' e₁ e₂) (ctx : Ctx) (HEnv : V' = ctx.updateEnv V)
-  (He₁ : e₁' = ctx.fill e₁) (He₂ : e₂' = ctx.fill e₂) : SmallStep defs V e₁' e₂' := by
-  rw [HEnv] at st
-  let result := SmallStep.ctx_step ctx V st
-  rw [← He₁, ← He₂] at result
-  assumption
+@[simp] lemma addBindings_single {e xe : Expr}
+    : e.addBindings [(x, xe)] = Expr.letIn x xe e := by sorry
 
-lemma steps_in_context_imply_steps_in_expr {e₁ e₂ e₁' e₂' : Expr} {V V' : Env} {defs : Definitions}
-  (sts : SmallSteps defs V' e₁ e₂) (ctx : Ctx) (HEnv : V' = ctx.updateEnv V)
-  (He₁ : e₁' = ctx.fill e₁) (He₂ : e₂' = ctx.fill e₂) : SmallSteps defs V e₁' e₂' := by sorry
+lemma SmallStep.hole_step : HeadSmallStep defs V e₁ e₂ → SmallStep defs V e₁ e₂ := by sorry
+
+lemma SmallStep.with_ctx (ctx : Ctx)
+    : (e₁' = ctx.fill e₁) → (e₂' = ctx.fill e₂)
+    → SmallStep defs (ctx.updateEnv V) e₁ e₂ → SmallStep defs V e₁' e₂' := by sorry
+
+lemma SmallSteps.with_ctx (ctx : Ctx)
+    : (e₁' = ctx.fill e₁) → (e₂' = ctx.fill e₂)
+    → SmallSteps defs (ctx.updateEnv V) e₁ e₂ → SmallSteps defs V e₁' e₂' := by sorry
